tests/IIR.bpl
@@ -11,6 +11,7 @@ var M: MType;
 var C: CType;
 var R: CType;
 var I: CType;
+var T: CType;
 
 const unique this#: Actor;
 type List a = [int]a;
@@ -332,39 +333,9 @@ procedure iir#init#10()
   assume 0 == 0;
   M[iir#f][C[iir#f]] := 0;
   C[iir#f] := C[iir#f] + 1;
-  assume M[iir#f][0] == 0;
-  assume R[iir#e] == (C[iir#f] - 1);
-  assume (forall idx$: int :: 
-    (1 <= idx$) && (idx$ < C[iir#f]) ==> (M[iir#f][idx$] == M[iir#e][idx$ - 1])
-  );
   assume 85 == 85;
-  assume R[iir#a] == C[iir#b];
-  assume (forall idx$: int :: 
-    (0 <= idx$) && (idx$ < C[iir#b]) ==> (M[iir#b][idx$] == (85 * M[iir#a][idx$]))
-  );
   assume 171 == 171;
-  assume R[iir#d] == C[iir#e];
-  assume (forall idx$: int :: 
-    (0 <= idx$) && (idx$ < C[iir#e]) ==> (M[iir#e][idx$] == (171 * M[iir#d][idx$]))
-  );
   assume 8 == 8;
-  assume R[iir#c] == C[iir#g];
-  assume (forall idx$: int :: 
-    (0 <= idx$) && (idx$ < C[iir#g]) ==> (M[iir#g][idx$] == AT#RShift(M[iir#c][idx$], 8))
-  );
-  assume R[iir#b] == C[iir#c];
-  assume R[iir#f] == C[iir#c];
-  assume (forall idx$: int :: 
-    (0 <= idx$) && (idx$ < C[iir#c]) ==> (M[iir#c][idx$] == (M[iir#b][idx$] + M[iir#f][idx$]))
-  );
-  assume R[iir#g] == C[iir#d];
-  assume R[iir#g] == C[iir#h];
-  assume (forall idx$: int :: 
-    (0 <= idx$) && (idx$ < C[iir#d]) ==> (M[iir#d][idx$] == M[iir#g][idx$])
-  );
-  assume (forall idx$: int :: 
-    (0 <= idx$) && (idx$ < C[iir#h]) ==> (M[iir#h][idx$] == M[iir#g][idx$])
-  );
   assert {:msg "Initialization of network 'iir' might not establish the channel invariant (#28)"} I[iir#f] == I[iir#e];
   assert {:msg "Initialization of network 'iir' might not establish the channel invariant (#29)"} I[iir#b] == I[iir#a];
   assert {:msg "Initialization of network 'iir' might not establish the channel invariant (#30)"} I[iir#e] == I[iir#d];
@@ -374,13 +345,12 @@ procedure iir#init#10()
   assert {:msg "Initialization of network 'iir' might not establish the channel invariant (#34)"} I[iir#d] == I[iir#g];
   assert {:msg "Initialization of network 'iir' might not establish the channel invariant (#35)"} I[iir#h] == I[iir#g];
   I := R;
-  C[iir#f] := C[iir#f] - 1;
-  assert {:msg "42.5: The initialization might produce unspecified tokens on channel a (#36)"} (C[iir#a] - R[iir#a]) == 0;
-  assert {:msg "43.5: The initialization might produce unspecified tokens on channel b (#37)"} (C[iir#b] - R[iir#b]) == 0;
-  assert {:msg "44.5: The initialization might produce unspecified tokens on channel c (#38)"} (C[iir#c] - R[iir#c]) == 0;
-  assert {:msg "45.5: The initialization might produce unspecified tokens on channel d (#39)"} (C[iir#d] - R[iir#d]) == 0;
-  assert {:msg "46.5: The initialization might produce unspecified tokens on channel e (#40)"} (C[iir#e] - R[iir#e]) == 0;
-  assert {:msg "47.5: The initialization might produce unspecified tokens on channel f (#41)"} (C[iir#f] - R[iir#f]) == 0;
+  assert {:msg "30.13: Network initialization might not establish the network invariant (#36)"} (C[iir#f] - R[iir#f]) == 1;
+  assert {:msg "42.5: The initialization might produce unspecified tokens on channel a (#37)"} (C[iir#a] - R[iir#a]) == 0;
+  assert {:msg "43.5: The initialization might produce unspecified tokens on channel b (#38)"} (C[iir#b] - R[iir#b]) == 0;
+  assert {:msg "44.5: The initialization might produce unspecified tokens on channel c (#39)"} (C[iir#c] - R[iir#c]) == 0;
+  assert {:msg "45.5: The initialization might produce unspecified tokens on channel d (#40)"} (C[iir#d] - R[iir#d]) == 0;
+  assert {:msg "46.5: The initialization might produce unspecified tokens on channel e (#41)"} (C[iir#e] - R[iir#e]) == 0;
   assert {:msg "48.5: The initialization might produce unspecified tokens on channel g (#42)"} (C[iir#g] - R[iir#g]) == 0;
   assert {:msg "49.5: The initialization might produce unspecified tokens on channel h (#43)"} (C[iir#h] - R[iir#h]) == 0;
 }
@@ -437,7 +407,6 @@ procedure iir##delay#anon$2#11()
   assume I[iir#c] == I[iir#f];
   assume I[iir#d] == I[iir#g];
   assume I[iir#h] == I[iir#g];
-  assume M[iir#f][0] == 0;
   assume R[iir#e] == (C[iir#f] - 1);
   assume (forall idx$: int :: 
     (1 <= idx$) && (idx$ < C[iir#f]) ==> (M[iir#f][idx$] == M[iir#e][idx$ - 1])
@@ -468,21 +437,10 @@ procedure iir##delay#anon$2#11()
     (0 <= idx$) && (idx$ < C[iir#h]) ==> (M[iir#h][idx$] == M[iir#g][idx$])
   );
   assume 1 <= (C[iir#e] - R[iir#e]);
-  assume M[iir#f][0] == 0;
-  assume R[iir#e] == (C[iir#f] - 1);
-  assume (forall idx$: int :: 
-    (1 <= idx$) && (idx$ < C[iir#f]) ==> (M[iir#f][idx$] == M[iir#e][idx$ - 1])
-  );
   in#i := M[iir#e][R[iir#e]];
   R[iir#e] := R[iir#e] + 1;
   M[iir#f][C[iir#f]] := in#i;
   C[iir#f] := C[iir#f] + 1;
-  assume M[iir#f][0] == 0;
-  assume R[iir#e] == (C[iir#f] - 1);
-  assume (forall idx$: int :: 
-    (1 <= idx$) && (idx$ < C[iir#f]) ==> (M[iir#f][idx$] == M[iir#e][idx$ - 1])
-  );
-  assume M[iir#f][0] == 0;
   assume R[iir#e] == (C[iir#f] - 1);
   assume (forall idx$: int :: 
     (1 <= idx$) && (idx$ < C[iir#f]) ==> (M[iir#f][idx$] == M[iir#e][idx$ - 1])
@@ -574,7 +532,6 @@ procedure iir##mulc#anon$3#12()
   assume I[iir#c] == I[iir#f];
   assume I[iir#d] == I[iir#g];
   assume I[iir#h] == I[iir#g];
-  assume M[iir#f][0] == 0;
   assume R[iir#e] == (C[iir#f] - 1);
   assume (forall idx$: int :: 
     (1 <= idx$) && (idx$ < C[iir#f]) ==> (M[iir#f][idx$] == M[iir#e][idx$ - 1])
@@ -605,19 +562,10 @@ procedure iir##mulc#anon$3#12()
     (0 <= idx$) && (idx$ < C[iir#h]) ==> (M[iir#h][idx$] == M[iir#g][idx$])
   );
   assume 1 <= (C[iir#a] - R[iir#a]);
-  assume R[iir#a] == C[iir#b];
-  assume (forall idx$: int :: 
-    (0 <= idx$) && (idx$ < C[iir#b]) ==> (M[iir#b][idx$] == (85 * M[iir#a][idx$]))
-  );
   in#i := M[iir#a][R[iir#a]];
   R[iir#a] := R[iir#a] + 1;
   M[iir#b][C[iir#b]] := 85 * in#i;
   C[iir#b] := C[iir#b] + 1;
-  assume R[iir#a] == C[iir#b];
-  assume (forall idx$: int :: 
-    (0 <= idx$) && (idx$ < C[iir#b]) ==> (M[iir#b][idx$] == (85 * M[iir#a][idx$]))
-  );
-  assume M[iir#f][0] == 0;
   assume R[iir#e] == (C[iir#f] - 1);
   assume (forall idx$: int :: 
     (1 <= idx$) && (idx$ < C[iir#f]) ==> (M[iir#f][idx$] == M[iir#e][idx$ - 1])
@@ -709,7 +657,6 @@ procedure iir##mulc#anon$3#13()
   assume I[iir#c] == I[iir#f];
   assume I[iir#d] == I[iir#g];
   assume I[iir#h] == I[iir#g];
-  assume M[iir#f][0] == 0;
   assume R[iir#e] == (C[iir#f] - 1);
   assume (forall idx$: int :: 
     (1 <= idx$) && (idx$ < C[iir#f]) ==> (M[iir#f][idx$] == M[iir#e][idx$ - 1])
@@ -740,19 +687,10 @@ procedure iir##mulc#anon$3#13()
     (0 <= idx$) && (idx$ < C[iir#h]) ==> (M[iir#h][idx$] == M[iir#g][idx$])
   );
   assume 1 <= (C[iir#d] - R[iir#d]);
-  assume R[iir#d] == C[iir#e];
-  assume (forall idx$: int :: 
-    (0 <= idx$) && (idx$ < C[iir#e]) ==> (M[iir#e][idx$] == (171 * M[iir#d][idx$]))
-  );
   in#i := M[iir#d][R[iir#d]];
   R[iir#d] := R[iir#d] + 1;
   M[iir#e][C[iir#e]] := 171 * in#i;
   C[iir#e] := C[iir#e] + 1;
-  assume R[iir#d] == C[iir#e];
-  assume (forall idx$: int :: 
-    (0 <= idx$) && (idx$ < C[iir#e]) ==> (M[iir#e][idx$] == (171 * M[iir#d][idx$]))
-  );
-  assume M[iir#f][0] == 0;
   assume R[iir#e] == (C[iir#f] - 1);
   assume (forall idx$: int :: 
     (1 <= idx$) && (idx$ < C[iir#f]) ==> (M[iir#f][idx$] == M[iir#e][idx$ - 1])
@@ -844,7 +782,6 @@ procedure iir##rshift#anon$4#14()
   assume I[iir#c] == I[iir#f];
   assume I[iir#d] == I[iir#g];
   assume I[iir#h] == I[iir#g];
-  assume M[iir#f][0] == 0;
   assume R[iir#e] == (C[iir#f] - 1);
   assume (forall idx$: int :: 
     (1 <= idx$) && (idx$ < C[iir#f]) ==> (M[iir#f][idx$] == M[iir#e][idx$ - 1])
@@ -875,19 +812,10 @@ procedure iir##rshift#anon$4#14()
     (0 <= idx$) && (idx$ < C[iir#h]) ==> (M[iir#h][idx$] == M[iir#g][idx$])
   );
   assume 1 <= (C[iir#c] - R[iir#c]);
-  assume R[iir#c] == C[iir#g];
-  assume (forall idx$: int :: 
-    (0 <= idx$) && (idx$ < C[iir#g]) ==> (M[iir#g][idx$] == AT#RShift(M[iir#c][idx$], 8))
-  );
   in#i := M[iir#c][R[iir#c]];
   R[iir#c] := R[iir#c] + 1;
   M[iir#g][C[iir#g]] := AT#RShift(in#i, 8);
   C[iir#g] := C[iir#g] + 1;
-  assume R[iir#c] == C[iir#g];
-  assume (forall idx$: int :: 
-    (0 <= idx$) && (idx$ < C[iir#g]) ==> (M[iir#g][idx$] == AT#RShift(M[iir#c][idx$], 8))
-  );
-  assume M[iir#f][0] == 0;
   assume R[iir#e] == (C[iir#f] - 1);
   assume (forall idx$: int :: 
     (1 <= idx$) && (idx$ < C[iir#f]) ==> (M[iir#f][idx$] == M[iir#e][idx$ - 1])
@@ -980,7 +908,6 @@ procedure iir##add#anon$0#15()
   assume I[iir#c] == I[iir#f];
   assume I[iir#d] == I[iir#g];
   assume I[iir#h] == I[iir#g];
-  assume M[iir#f][0] == 0;
   assume R[iir#e] == (C[iir#f] - 1);
   assume (forall idx$: int :: 
     (1 <= idx$) && (idx$ < C[iir#f]) ==> (M[iir#f][idx$] == M[iir#e][idx$ - 1])
@@ -1011,23 +938,12 @@ procedure iir##add#anon$0#15()
     (0 <= idx$) && (idx$ < C[iir#h]) ==> (M[iir#h][idx$] == M[iir#g][idx$])
   );
   assume (1 <= (C[iir#b] - R[iir#b])) && (1 <= (C[iir#f] - R[iir#f]));
-  assume R[iir#b] == C[iir#c];
-  assume R[iir#f] == C[iir#c];
-  assume (forall idx$: int :: 
-    (0 <= idx$) && (idx$ < C[iir#c]) ==> (M[iir#c][idx$] == (M[iir#b][idx$] + M[iir#f][idx$]))
-  );
   in1#i := M[iir#b][R[iir#b]];
   R[iir#b] := R[iir#b] + 1;
   in2#j := M[iir#f][R[iir#f]];
   R[iir#f] := R[iir#f] + 1;
   M[iir#c][C[iir#c]] := in1#i + in2#j;
   C[iir#c] := C[iir#c] + 1;
-  assume R[iir#b] == C[iir#c];
-  assume R[iir#f] == C[iir#c];
-  assume (forall idx$: int :: 
-    (0 <= idx$) && (idx$ < C[iir#c]) ==> (M[iir#c][idx$] == (M[iir#b][idx$] + M[iir#f][idx$]))
-  );
-  assume M[iir#f][0] == 0;
   assume R[iir#e] == (C[iir#f] - 1);
   assume (forall idx$: int :: 
     (1 <= idx$) && (idx$ < C[iir#f]) ==> (M[iir#f][idx$] == M[iir#e][idx$ - 1])
@@ -1119,7 +1035,6 @@ procedure iir##split#anon$5#16()
   assume I[iir#c] == I[iir#f];
   assume I[iir#d] == I[iir#g];
   assume I[iir#h] == I[iir#g];
-  assume M[iir#f][0] == 0;
   assume R[iir#e] == (C[iir#f] - 1);
   assume (forall idx$: int :: 
     (1 <= idx$) && (idx$ < C[iir#f]) ==> (M[iir#f][idx$] == M[iir#e][idx$ - 1])
@@ -1150,29 +1065,12 @@ procedure iir##split#anon$5#16()
     (0 <= idx$) && (idx$ < C[iir#h]) ==> (M[iir#h][idx$] == M[iir#g][idx$])
   );
   assume 1 <= (C[iir#g] - R[iir#g]);
-  assume R[iir#g] == C[iir#d];
-  assume R[iir#g] == C[iir#h];
-  assume (forall idx$: int :: 
-    (0 <= idx$) && (idx$ < C[iir#d]) ==> (M[iir#d][idx$] == M[iir#g][idx$])
-  );
-  assume (forall idx$: int :: 
-    (0 <= idx$) && (idx$ < C[iir#h]) ==> (M[iir#h][idx$] == M[iir#g][idx$])
-  );
   in#i := M[iir#g][R[iir#g]];
   R[iir#g] := R[iir#g] + 1;
   M[iir#d][C[iir#d]] := in#i;
   C[iir#d] := C[iir#d] + 1;
   M[iir#h][C[iir#h]] := in#i;
   C[iir#h] := C[iir#h] + 1;
-  assume R[iir#g] == C[iir#d];
-  assume R[iir#g] == C[iir#h];
-  assume (forall idx$: int :: 
-    (0 <= idx$) && (idx$ < C[iir#d]) ==> (M[iir#d][idx$] == M[iir#g][idx$])
-  );
-  assume (forall idx$: int :: 
-    (0 <= idx$) && (idx$ < C[iir#h]) ==> (M[iir#h][idx$] == M[iir#g][idx$])
-  );
-  assume M[iir#f][0] == 0;
   assume R[iir#e] == (C[iir#f] - 1);
   assume (forall idx$: int :: 
     (1 <= idx$) && (idx$ < C[iir#f]) ==> (M[iir#f][idx$] == M[iir#e][idx$ - 1])
@@ -1211,104 +1109,6 @@ procedure iir##split#anon$5#16()
   assert {:msg "Action at 20.3 ('anon$5') for actor instance 'spl1' might not preserve the channel invariant (#90)"} I[iir#d] == I[iir#g];
   assert {:msg "Action at 20.3 ('anon$5') for actor instance 'spl1' might not preserve the channel invariant (#91)"} I[iir#h] == I[iir#g];
 }
-procedure iir#entry()
-  modifies C, R, M, I;
-{
-  var iir#del1: Actor;
-  var iir#mul1: Actor;
-  var iir#mul2: Actor;
-  var iir#rsh1: Actor;
-  var iir#add1: Actor;
-  var iir#spl1: Actor;
-  var iir#a: Chan (int);
-  var iir#b: Chan (int);
-  var iir#c: Chan (int);
-  var iir#d: Chan (int);
-  var iir#e: Chan (int);
-  var iir#f: Chan (int);
-  var iir#g: Chan (int);
-  var iir#h: Chan (int);
-  assume (iir#del1 != iir#mul1) && (iir#del1 != iir#mul2) && (iir#del1 != iir#rsh1) && (iir#del1 != iir#add1) && (iir#del1 != iir#spl1) && (iir#mul1 != iir#mul2) && (iir#mul1 != iir#rsh1) && (iir#mul1 != iir#add1) && (iir#mul1 != iir#spl1) && (iir#mul2 != iir#rsh1) && (iir#mul2 != iir#add1) && (iir#mul2 != iir#spl1) && (iir#rsh1 != iir#add1) && (iir#rsh1 != iir#spl1) && (iir#add1 != iir#spl1);
-  assume (iir#a != iir#b) && (iir#a != iir#c) && (iir#a != iir#d) && (iir#a != iir#e) && (iir#a != iir#f) && (iir#a != iir#g) && (iir#a != iir#h) && (iir#b != iir#c) && (iir#b != iir#d) && (iir#b != iir#e) && (iir#b != iir#f) && (iir#b != iir#g) && (iir#b != iir#h) && (iir#c != iir#d) && (iir#c != iir#e) && (iir#c != iir#f) && (iir#c != iir#g) && (iir#c != iir#h) && (iir#d != iir#e) && (iir#d != iir#f) && (iir#d != iir#g) && (iir#d != iir#h) && (iir#e != iir#f) && (iir#e != iir#g) && (iir#e != iir#h) && (iir#f != iir#g) && (iir#f != iir#h) && (iir#g != iir#h);
-  assume 0 <= I[iir#a];
-  assume I[iir#a] <= R[iir#a];
-  assume R[iir#a] <= C[iir#a];
-  assume 0 <= I[iir#b];
-  assume I[iir#b] <= R[iir#b];
-  assume R[iir#b] <= C[iir#b];
-  assume 0 <= I[iir#c];
-  assume I[iir#c] <= R[iir#c];
-  assume R[iir#c] <= C[iir#c];
-  assume 0 <= I[iir#d];
-  assume I[iir#d] <= R[iir#d];
-  assume R[iir#d] <= C[iir#d];
-  assume 0 <= I[iir#e];
-  assume I[iir#e] <= R[iir#e];
-  assume R[iir#e] <= C[iir#e];
-  assume 0 <= I[iir#f];
-  assume I[iir#f] <= R[iir#f];
-  assume R[iir#f] <= C[iir#f];
-  assume 0 <= I[iir#g];
-  assume I[iir#g] <= R[iir#g];
-  assume R[iir#g] <= C[iir#g];
-  assume 0 <= I[iir#h];
-  assume I[iir#h] <= R[iir#h];
-  assume R[iir#h] <= C[iir#h];
-  assume I[iir#h] == R[iir#h];
-  assume C[iir#a] == R[iir#a];
-  assume C[iir#b] == R[iir#b];
-  assume C[iir#c] == R[iir#c];
-  assume C[iir#d] == R[iir#d];
-  assume C[iir#e] == R[iir#e];
-  assume C[iir#f] == R[iir#f];
-  assume C[iir#g] == R[iir#g];
-  assume C[iir#h] == R[iir#h];
-  C[iir#f] := C[iir#f] + 1;
-  assume I[iir#f] == I[iir#e];
-  assume I[iir#b] == I[iir#a];
-  assume I[iir#e] == I[iir#d];
-  assume I[iir#g] == I[iir#c];
-  assume I[iir#c] == I[iir#b];
-  assume I[iir#c] == I[iir#f];
-  assume I[iir#d] == I[iir#g];
-  assume I[iir#h] == I[iir#g];
-  assume M[iir#f][0] == 0;
-  assume R[iir#e] == (C[iir#f] - 1);
-  assume (forall idx$: int :: 
-    (1 <= idx$) && (idx$ < C[iir#f]) ==> (M[iir#f][idx$] == M[iir#e][idx$ - 1])
-  );
-  assume R[iir#a] == C[iir#b];
-  assume (forall idx$: int :: 
-    (0 <= idx$) && (idx$ < C[iir#b]) ==> (M[iir#b][idx$] == (85 * M[iir#a][idx$]))
-  );
-  assume R[iir#d] == C[iir#e];
-  assume (forall idx$: int :: 
-    (0 <= idx$) && (idx$ < C[iir#e]) ==> (M[iir#e][idx$] == (171 * M[iir#d][idx$]))
-  );
-  assume R[iir#c] == C[iir#g];
-  assume (forall idx$: int :: 
-    (0 <= idx$) && (idx$ < C[iir#g]) ==> (M[iir#g][idx$] == AT#RShift(M[iir#c][idx$], 8))
-  );
-  assume R[iir#b] == C[iir#c];
-  assume R[iir#f] == C[iir#c];
-  assume (forall idx$: int :: 
-    (0 <= idx$) && (idx$ < C[iir#c]) ==> (M[iir#c][idx$] == (M[iir#b][idx$] + M[iir#f][idx$]))
-  );
-  assume R[iir#g] == C[iir#d];
-  assume R[iir#g] == C[iir#h];
-  assume (forall idx$: int :: 
-    (0 <= idx$) && (idx$ < C[iir#d]) ==> (M[iir#d][idx$] == M[iir#g][idx$])
-  );
-  assume (forall idx$: int :: 
-    (0 <= idx$) && (idx$ < C[iir#h]) ==> (M[iir#h][idx$] == M[iir#g][idx$])
-  );
-  assert {:msg "23.1: Sub-actors in the network might fire without network input. This is not permitted. (#92)"} !(1 <= (C[iir#e] - R[iir#e]));
-  assert {:msg "23.1: Sub-actors in the network might fire without network input. This is not permitted. (#93)"} !(1 <= (C[iir#a] - R[iir#a]));
-  assert {:msg "23.1: Sub-actors in the network might fire without network input. This is not permitted. (#94)"} !(1 <= (C[iir#d] - R[iir#d]));
-  assert {:msg "23.1: Sub-actors in the network might fire without network input. This is not permitted. (#95)"} !(1 <= (C[iir#c] - R[iir#c]));
-  assert {:msg "23.1: Sub-actors in the network might fire without network input. This is not permitted. (#96)"} !((1 <= (C[iir#b] - R[iir#b])) && (1 <= (C[iir#f] - R[iir#f])));
-  assert {:msg "23.1: Sub-actors in the network might fire without network input. This is not permitted. (#97)"} !(1 <= (C[iir#g] - R[iir#g]));
-}
 procedure iir#anon$6#input#in#17()
   modifies C, R, M, I;
 {
@@ -1326,7 +1126,6 @@ procedure iir#anon$6#input#in#17()
   var iir#f: Chan (int);
   var iir#g: Chan (int);
   var iir#h: Chan (int);
-  var x: int;
   assume (iir#del1 != iir#mul1) && (iir#del1 != iir#mul2) && (iir#del1 != iir#rsh1) && (iir#del1 != iir#add1) && (iir#del1 != iir#spl1) && (iir#mul1 != iir#mul2) && (iir#mul1 != iir#rsh1) && (iir#mul1 != iir#add1) && (iir#mul1 != iir#spl1) && (iir#mul2 != iir#rsh1) && (iir#mul2 != iir#add1) && (iir#mul2 != iir#spl1) && (iir#rsh1 != iir#add1) && (iir#rsh1 != iir#spl1) && (iir#add1 != iir#spl1);
   assume (iir#a != iir#b) && (iir#a != iir#c) && (iir#a != iir#d) && (iir#a != iir#e) && (iir#a != iir#f) && (iir#a != iir#g) && (iir#a != iir#h) && (iir#b != iir#c) && (iir#b != iir#d) && (iir#b != iir#e) && (iir#b != iir#f) && (iir#b != iir#g) && (iir#b != iir#h) && (iir#c != iir#d) && (iir#c != iir#e) && (iir#c != iir#f) && (iir#c != iir#g) && (iir#c != iir#h) && (iir#d != iir#e) && (iir#d != iir#f) && (iir#d != iir#g) && (iir#d != iir#h) && (iir#e != iir#f) && (iir#e != iir#g) && (iir#e != iir#h) && (iir#f != iir#g) && (iir#f != iir#h) && (iir#g != iir#h);
   assume 0 <= I[iir#a];
@@ -1354,6 +1153,7 @@ procedure iir#anon$6#input#in#17()
   assume I[iir#h] <= R[iir#h];
   assume R[iir#h] <= C[iir#h];
   assume I[iir#h] == R[iir#h];
+  assume (C[iir#a] - I[iir#a]) < 1;
   assume I[iir#f] == I[iir#e];
   assume I[iir#b] == I[iir#a];
   assume I[iir#e] == I[iir#d];
@@ -1362,7 +1162,6 @@ procedure iir#anon$6#input#in#17()
   assume I[iir#c] == I[iir#f];
   assume I[iir#d] == I[iir#g];
   assume I[iir#h] == I[iir#g];
-  assume M[iir#f][0] == 0;
   assume R[iir#e] == (C[iir#f] - 1);
   assume (forall idx$: int :: 
     (1 <= idx$) && (idx$ < C[iir#f]) ==> (M[iir#f][idx$] == M[iir#e][idx$ - 1])
@@ -1392,16 +1191,15 @@ procedure iir#anon$6#input#in#17()
   assume (forall idx$: int :: 
     (0 <= idx$) && (idx$ < C[iir#h]) ==> (M[iir#h][idx$] == M[iir#g][idx$])
   );
-  assume 0 <= x;
-  C[iir#a] := C[iir#a] + x;
-  assert {:msg "Channel invariant might be falsified by network input (#98)"} I[iir#f] == I[iir#e];
-  assert {:msg "Channel invariant might be falsified by network input (#99)"} I[iir#b] == I[iir#a];
-  assert {:msg "Channel invariant might be falsified by network input (#100)"} I[iir#e] == I[iir#d];
-  assert {:msg "Channel invariant might be falsified by network input (#101)"} I[iir#g] == I[iir#c];
-  assert {:msg "Channel invariant might be falsified by network input (#102)"} I[iir#c] == I[iir#b];
-  assert {:msg "Channel invariant might be falsified by network input (#103)"} I[iir#c] == I[iir#f];
-  assert {:msg "Channel invariant might be falsified by network input (#104)"} I[iir#d] == I[iir#g];
-  assert {:msg "Channel invariant might be falsified by network input (#105)"} I[iir#h] == I[iir#g];
+  C[iir#a] := C[iir#a] + 1;
+  assert {:msg "Channel invariant might be falsified by network input (#92)"} I[iir#f] == I[iir#e];
+  assert {:msg "Channel invariant might be falsified by network input (#93)"} I[iir#b] == I[iir#a];
+  assert {:msg "Channel invariant might be falsified by network input (#94)"} I[iir#e] == I[iir#d];
+  assert {:msg "Channel invariant might be falsified by network input (#95)"} I[iir#g] == I[iir#c];
+  assert {:msg "Channel invariant might be falsified by network input (#96)"} I[iir#c] == I[iir#b];
+  assert {:msg "Channel invariant might be falsified by network input (#97)"} I[iir#c] == I[iir#f];
+  assert {:msg "Channel invariant might be falsified by network input (#98)"} I[iir#d] == I[iir#g];
+  assert {:msg "Channel invariant might be falsified by network input (#99)"} I[iir#h] == I[iir#g];
 }
 procedure iir#anon$6#exit#18()
   modifies C, R, M, I;
@@ -1455,7 +1253,6 @@ procedure iir#anon$6#exit#18()
   assume I[iir#c] == I[iir#f];
   assume I[iir#d] == I[iir#g];
   assume I[iir#h] == I[iir#g];
-  assume M[iir#f][0] == 0;
   assume R[iir#e] == (C[iir#f] - 1);
   assume (forall idx$: int :: 
     (1 <= idx$) && (idx$ < C[iir#f]) ==> (M[iir#f][idx$] == M[iir#e][idx$ - 1])
@@ -1492,25 +1289,24 @@ procedure iir#anon$6#exit#18()
   assume !(1 <= (C[iir#c] - R[iir#c]));
   assume !((1 <= (C[iir#b] - R[iir#b])) && (1 <= (C[iir#f] - R[iir#f])));
   assume !(1 <= (C[iir#g] - R[iir#g]));
-  assert {:msg "26.13: Network action postcondition might not hold (#106)"} M[iir#h][0] == AT#RShift(85 * M[iir#a][0], 8);
-  assert {:msg "27.13: Network action postcondition might not hold (#107)"} (0 < I[iir#h]) ==> (M[iir#h][I[iir#h]] == AT#RShift((171 * M[iir#h][I[iir#h] - 1]) + (85 * M[iir#a][I[iir#a]]), 8));
+  assert {:msg "26.13: Network action postcondition might not hold (#100)"} M[iir#h][0] == AT#RShift(85 * M[iir#a][0], 8);
+  assert {:msg "27.13: Network action postcondition might not hold (#101)"} (0 < I[iir#h]) ==> (M[iir#h][I[iir#h]] == AT#RShift((171 * M[iir#h][I[iir#h] - 1]) + (85 * M[iir#a][I[iir#a]]), 8));
   R[iir#h] := R[iir#h] + 1;
   I := R;
-  assert {:msg "The network might not preserve the channel invariant (#108)"} I[iir#f] == I[iir#e];
-  assert {:msg "The network might not preserve the channel invariant (#109)"} I[iir#b] == I[iir#a];
-  assert {:msg "The network might not preserve the channel invariant (#110)"} I[iir#e] == I[iir#d];
-  assert {:msg "The network might not preserve the channel invariant (#111)"} I[iir#g] == I[iir#c];
-  assert {:msg "The network might not preserve the channel invariant (#112)"} I[iir#c] == I[iir#b];
-  assert {:msg "The network might not preserve the channel invariant (#113)"} I[iir#c] == I[iir#f];
-  assert {:msg "The network might not preserve the channel invariant (#114)"} I[iir#d] == I[iir#g];
-  assert {:msg "The network might not preserve the channel invariant (#115)"} I[iir#h] == I[iir#g];
-  C[iir#f] := C[iir#f] - 1;
-  assert {:msg "25.3: The network might leave unread tokens on channel a (#116)"} C[iir#a] == R[iir#a];
-  assert {:msg "25.3: The network might leave unread tokens on channel b (#117)"} C[iir#b] == R[iir#b];
-  assert {:msg "25.3: The network might leave unread tokens on channel c (#118)"} C[iir#c] == R[iir#c];
-  assert {:msg "25.3: The network might leave unread tokens on channel d (#119)"} C[iir#d] == R[iir#d];
-  assert {:msg "25.3: The network might leave unread tokens on channel e (#120)"} C[iir#e] == R[iir#e];
-  assert {:msg "25.3: The network might leave unread tokens on channel f (#121)"} C[iir#f] == R[iir#f];
-  assert {:msg "25.3: The network might leave unread tokens on channel g (#122)"} C[iir#g] == R[iir#g];
-  assert {:msg "25.3: The network might not produce the specified number of tokens on output out (#123)"} C[iir#h] == R[iir#h];
+  assert {:msg "The network might not preserve the channel invariant (#102)"} I[iir#f] == I[iir#e];
+  assert {:msg "The network might not preserve the channel invariant (#103)"} I[iir#b] == I[iir#a];
+  assert {:msg "The network might not preserve the channel invariant (#104)"} I[iir#e] == I[iir#d];
+  assert {:msg "The network might not preserve the channel invariant (#105)"} I[iir#g] == I[iir#c];
+  assert {:msg "The network might not preserve the channel invariant (#106)"} I[iir#c] == I[iir#b];
+  assert {:msg "The network might not preserve the channel invariant (#107)"} I[iir#c] == I[iir#f];
+  assert {:msg "The network might not preserve the channel invariant (#108)"} I[iir#d] == I[iir#g];
+  assert {:msg "The network might not preserve the channel invariant (#109)"} I[iir#h] == I[iir#g];
+  assert {:msg "30.13: The network might not preserve the network invariant (#110)"} (C[iir#f] - R[iir#f]) == 1;
+  assert {:msg "25.3: The network might leave unread tokens on channel a (#111)"} (C[iir#a] - R[iir#a]) == 0;
+  assert {:msg "25.3: The network might leave unread tokens on channel b (#112)"} (C[iir#b] - R[iir#b]) == 0;
+  assert {:msg "25.3: The network might leave unread tokens on channel c (#113)"} (C[iir#c] - R[iir#c]) == 0;
+  assert {:msg "25.3: The network might leave unread tokens on channel d (#114)"} (C[iir#d] - R[iir#d]) == 0;
+  assert {:msg "25.3: The network might leave unread tokens on channel e (#115)"} (C[iir#e] - R[iir#e]) == 0;
+  assert {:msg "25.3: The network might leave unread tokens on channel g (#116)"} (C[iir#g] - R[iir#g]) == 0;
+  assert {:msg "25.3: The network might not produce the specified number of tokens on output out (#117)"} (C[iir#h] - R[iir#h]) == 0;
 }
